Weidenbach_Book/IsaSAT/IsaSAT_Bump_Heuristics_State.thy
@@ -24,6 +24,9 @@ abbreviation get_focused_heuristics :: \<open>bump_heuristics \<Rightarrow> vmtf
 abbreviation is_focused_heuristics :: \<open>bump_heuristics \<Rightarrow> bool\<close> where
   \<open>is_focused_heuristics \<equiv> Tuple4_c\<close>
 
+abbreviation is_stable_heuristics:: \<open>bump_heuristics \<Rightarrow> bool\<close> where
+  \<open>is_stable_heuristics x \<equiv> \<not>is_focused_heuristics x\<close>
+
 abbreviation get_bumped_variables :: \<open>bump_heuristics \<Rightarrow> nat list \<times> bool list\<close> where
   \<open>get_bumped_variables \<equiv> Tuple4_d\<close>
 
@@ -39,21 +42,28 @@ abbreviation set_is_focused_heuristics :: \<open>bool \<Rightarrow>bump_heuristi
 abbreviation set_bumped_variables :: \<open>nat list \<times> bool list \<Rightarrow>bump_heuristics \<Rightarrow> _\<close> where
   \<open>set_bumped_variables \<equiv> Tuple4.set_d\<close>
 
+definition get_unit_trail where
+  \<open>get_unit_trail M = (rev (takeWhile (\<lambda>x. \<not>is_decided x) (rev M)))\<close>
+
 definition bump_heur :: \<open>_ \<Rightarrow> _ \<Rightarrow> bump_heuristics set\<close> where
   \<open>bump_heur \<A> M = {x.
-    is_focused_heuristics x \<longrightarrow>
+    (is_focused_heuristics x \<longrightarrow>
+      (get_stable_heuristics x \<in> vmtf \<A> (get_unit_trail M)  \<and>
+      get_focused_heuristics x \<in> vmtf \<A> M)) \<and>
+    (\<not>is_focused_heuristics x \<longrightarrow>
       (get_stable_heuristics x \<in> vmtf \<A> M \<and>
-      get_focused_heuristics x \<in> vmtf \<A> (takeWhile (\<lambda>x. \<not>is_decided x) M)) \<and>
-    \<not>is_focused_heuristics x \<longrightarrow>
-      (get_stable_heuristics x \<in> vmtf \<A> (takeWhile (\<lambda>x. \<not>is_decided x) M) \<and>
-       get_focused_heuristics x \<in> vmtf \<A> M) \<and>
-  (get_bumped_variables x, set (fst (get_bumped_variables x))) \<in> distinct_atoms_rel \<A>
+       get_focused_heuristics x \<in> vmtf \<A> (get_unit_trail M))) \<and>
+   (get_bumped_variables x, set (fst (get_bumped_variables x))) \<in> distinct_atoms_rel \<A>
   }\<close>
 
 definition switch_bump_heur :: \<open>bump_heuristics \<Rightarrow> bump_heuristics\<close> where
   \<open>switch_bump_heur x = do {
     (set_is_focused_heuristics (\<not>(is_focused_heuristics x)) x)
   }\<close>
+
+lemma get_unit_trail_count_decided_0[simp]: \<open>count_decided M = 0 \<Longrightarrow> get_unit_trail M = M\<close>
+  by (auto simp: get_unit_trail_def count_decided_0_iff)
+   (metis rev_swap set_rev takeWhile_eq_all_conv)
 
 lemma switch_bump_heur:
   assumes \<open>x \<in> bump_heur \<A> M\<close> and
@@ -71,25 +81,45 @@ definition isa_vmtf_unset :: \<open>nat \<Rightarrow> bump_heuristics \<Rightarr
     (if foc then vmtf_unset L focused else focused)
     foc a)\<close>
 
+lemma get_unit_trail_simps[simp]: \<open>is_decided L \<Longrightarrow> get_unit_trail (L # M) = get_unit_trail M\<close>
+  \<open>\<not>is_decided L \<Longrightarrow> count_decided M = 0 \<Longrightarrow> get_unit_trail (L # M) = L # M\<close>
+  \<open>\<not>is_decided L \<Longrightarrow> count_decided M > 0 \<Longrightarrow> get_unit_trail (L # M) = get_unit_trail M\<close>
+  apply (auto simp: get_unit_trail_def takeWhile_append)
+  apply (metis set_rev takeWhile_eq_all_conv)
+  apply (metis count_decided_0_iff nat_neq_iff)
+  using bot_nat_0.not_eq_extremum count_decided_0_iff by blast
+
+lemma get_unit_trail_cons_if:
+  \<open>get_unit_trail (L # M) = (if is_decided L then get_unit_trail M else if count_decided M = 0 then L # M else get_unit_trail M)\<close>
+  by (auto simp: takeWhile_append)
+
+lemma get_unit_trail_tl[simp]: \<open>count_decided M > 0 \<Longrightarrow> get_unit_trail (tl M) = get_unit_trail M\<close>
+  by (cases M; cases \<open>hd M\<close>) auto
+
 lemma isa_vmtf_consD:
   \<open>x \<in> bump_heur \<A> M \<Longrightarrow> x \<in> bump_heur \<A> (L # M)\<close>
-  by (auto simp: bump_heur_def dest: vmtf_consD)
+  by (auto simp add: bump_heur_def takeWhile_append get_unit_trail_cons_if
+      intro!: vmtf_consD')
 
+lemma is_focused_heuristics_isa_vmtf_unset[simp]:
+  \<open>is_focused_heuristics (isa_vmtf_unset L x) = is_focused_heuristics x\<close>
+  by (auto simp: isa_vmtf_unset_def split: bump_heuristics_splits)
 
 lemma isa_vmtf_unset_vmtf_tl:
   fixes M
   defines [simp]: \<open>L \<equiv> atm_of (lit_of (hd M))\<close>
-  assumes vmtf:\<open>x\<in> bump_heur \<A> M\<close> and
-    L_N: \<open>L \<in> atms_of (\<L>\<^sub>a\<^sub>l\<^sub>l \<A>)\<close> and [simp]: \<open>M \<noteq> []\<close>
+  assumes vmtf: \<open>x\<in> bump_heur \<A> M\<close> and
+    L_N: \<open>L \<in> atms_of (\<L>\<^sub>a\<^sub>l\<^sub>l \<A>)\<close> and [simp]: \<open>M \<noteq> []\<close> and
+    nz: \<open>count_decided M > 0\<close>
   shows \<open>isa_vmtf_unset L x \<in> bump_heur \<A> (tl M)\<close>
 proof -
-  obtain ns m fst_As lst_As next_search remove where
+  obtain ns m fst_As lst_As next_search where
     \<open>is_focused_heuristics x \<Longrightarrow> get_focused_heuristics x = ((ns, m, fst_As, lst_As, next_search))\<close>
     \<open>\<not>is_focused_heuristics x \<Longrightarrow> get_stable_heuristics x = ((ns, m, fst_As, lst_As, next_search))\<close>
    by (cases \<open>get_focused_heuristics x\<close>; cases \<open>get_stable_heuristics x\<close>; cases \<open>is_focused_heuristics x\<close>) auto
-  show ?thesis
-    using vmtf_unset_vmtf_tl[of ns m fst_As lst_As next_search \<A> M]
-      assms by (auto simp: bump_heur_def)
+  then show ?thesis
+    using vmtf_unset_vmtf_tl[of ns m fst_As lst_As next_search \<A> M] nz
+      assms by (auto simp: bump_heur_def isa_vmtf_unset_def split: bump_heuristics_splits)
 qed
 
 end
